add a section about Stellar's intact sets

thys/Stellar_Quorums/Stellar_Quorums.thy
@@ -357,7 +357,7 @@ proof (rule ccontr)
     by (metis Int_commute inf_sup_aci(2) quorum_of_set_def) 
 qed
 
-section \<open>Reachability through a set\<close>
+subsection \<open>Reachability through a set\<close>
 
 text \<open>Here we define the part of a quorum @{term Q} of @{term p} that is reachable through correct
 participants from @{term p}. We show that if @{term p} and @{term p'} are members of the same consensus cluster and @{term Q} is a quorum of @{term p}
@@ -399,7 +399,7 @@ qed
 
 end
 
-section "Elementary quorums"
+subsection "Elementary quorums"
 
 text \<open>In this section we define the notion of elementary quorum, which is a quorum that has no strict subset that is a quorum.
   It follows directly from the definition that every finite quorum contains an elementary quorum. Moreover, we show 
@@ -474,6 +474,136 @@ proof -
       using elementary_def by auto
   }
   thus ?P by blast  
+qed
+
+
+end
+
+subsection \<open>The intact sets of the Stellar Whitepaper\<close>
+
+definition project where 
+  "project slices S n \<equiv> {Sl \<inter> S | Sl . Sl \<in> slices n}" 
+  \<comment> \<open>Projecting on @{term S} is the same as deleting the complement of @{term S}, where deleting is understood as in the Stellar Whitepaper.\<close>
+
+subsubsection \<open>Intact and the Cascade Theorem\<close>
+
+locale intact = \<comment> \<open>Here we fix an intact set @{term I} and prove the cascade theorem.\<close>
+  orig:stellar slices W 
+  + proj:stellar "project slices I" W \<comment> \<open>We consider the projection of the system on @{term I}.\<close>
+  for slices W I +  \<comment> \<open>An intact set is a set @{term I} satisfying the three assumptions below:\<close>
+  assumes intact_wb:"I \<subseteq> W"
+    and q_avail:"orig.quorum I" \<comment> \<open>@{term I} is a quorum in the original system.\<close>
+    and q_inter:"\<And> Q Q' . \<lbrakk>proj.quorum Q; proj.quorum Q'; Q \<inter> I \<noteq> {}; Q' \<inter> I \<noteq> {}\<rbrakk>  \<Longrightarrow> Q \<inter> Q' \<inter> I \<noteq> {}" 
+    \<comment> \<open>Any two sets that intersect @{term I} and that are quorums in the projected system intersect in @{term I}.
+Note that requiring that @{text \<open>Q \<inter> Q' \<noteq> {}\<close>} instead of @{text \<open>Q \<inter> Q' \<inter> I \<noteq> {}\<close>} would be equivalent.\<close>
+begin
+
+theorem blocking_safe: \<comment> \<open>A set that blocks an intact node contains an intact node. 
+If this were not the case, quorum availability would trivially be violated.\<close>
+  fixes S n
+  assumes "n\<in>I" and "\<forall> Sl\<in> slices n .Sl\<inter>S \<noteq> {}"
+  shows "S \<inter> I \<noteq> {}"
+  using assms q_avail intact_wb unfolding orig.quorum_def 
+  by auto (metis inf.absorb_iff2 inf_assoc inf_bot_right inf_sup_aci(1)) 
+
+theorem cascade:
+\<comment> \<open>If @{term U} is a quorum of an intact node and @{term S} is a super-set of @{term U}, then either @{term S} includes 
+all intact nodes or there is an intact node outside of @{term S} which is blocked by the intact members of @{term S}.
+This shows that, in SCP, once the intact members of a quorum accept a statement, 
+a cascading effect occurs and all intact nodes eventually accept it regardless of what befouled and faulty nodes do.\<close>
+  fixes U S
+  assumes "orig.quorum U" and "U \<inter> I \<noteq> {}" and "U \<subseteq> S"
+  obtains "I \<subseteq> S" | "\<exists> n \<in> I - S . \<forall> Sl \<in> slices n . Sl \<inter> S \<inter> I \<noteq> {}"
+proof -
+  have False if 1:"\<forall> n \<in> I - S . \<exists> Sl \<in> slices n . Sl \<inter> S \<inter> I = {}" and 2:"\<not>(I \<subseteq> S)"
+  proof -
+    text \<open>First we show that @{term \<open>I-S\<close>} is a quorum in the projected system. This is immediate from the definition of quorum and assumption 1.\<close>
+    have "proj.quorum (I-S)" using 1
+      unfolding proj.quorum_def project_def 
+      by (auto; smt DiffI Diff_Compl Diff_Int_distrib Diff_eq Diff_eq_empty_iff Int_commute)
+    text \<open>Then we show that U is also a quorum in the projected system:\<close>
+    moreover have "proj.quorum U" using \<open>orig.quorum U\<close> 
+      unfolding proj.quorum_def orig.quorum_def project_def 
+      by (simp; meson Int_commute inf.coboundedI2)
+    text \<open>Since quorums of @{term I} must intersect, we get a contradiction:\<close>
+    ultimately show False using \<open>U \<subseteq> S\<close> \<open>U \<inter> I \<noteq> {}\<close> \<open>\<not>(I\<subseteq>S)\<close> q_inter by auto
+  qed
+  thus ?thesis using that by blast
+qed
+
+end
+
+subsubsection "The Union Theorem"
+
+text \<open>Here we prove that the union of two intact sets that intersect is intact.
+This implies that maximal intact sets are disjoint.\<close>
+
+locale intersecting_intact = 
+  i1:intact slices W I\<^sub>1 + i2:intact slices W I\<^sub>2 \<comment> \<open>We fix two intersecting intact sets @{term I\<^sub>1} and @{term I\<^sub>2}.\<close>
+  + proj:stellar "project slices (I\<^sub>1\<union>I\<^sub>2)" W \<comment> \<open>We consider the projection of the system on @{term \<open>I\<^sub>1\<union>I\<^sub>2\<close>}.\<close>
+  for slices W I\<^sub>1 I\<^sub>2 +
+assumes inter:"I\<^sub>1 \<inter> I\<^sub>2 \<noteq> {}"
+begin
+
+theorem union_quorum: "i1.orig.quorum (I\<^sub>1\<union>I\<^sub>2)" \<comment> \<open>@{term \<open>I\<^sub>1\<union>I\<^sub>2\<close>} is a quorum in the original system.\<close>
+  using i1.intact_axioms i2.intact_axioms
+  unfolding  intact_def stellar_def intact_axioms_def i1.orig.quorum_def
+  by (metis Int_iff Un_iff le_supI1 le_supI2)
+
+theorem union_quorum_intersection: 
+  assumes "proj.quorum Q\<^sub>1" and "proj.quorum Q\<^sub>2" and "Q\<^sub>1 \<inter> (I\<^sub>1\<union>I\<^sub>2) \<noteq> {}" and "Q\<^sub>2 \<inter> (I\<^sub>1\<union>I\<^sub>2) \<noteq> {}"
+  shows "Q\<^sub>1 \<inter> Q\<^sub>2 \<inter> (I\<^sub>1\<union>I\<^sub>2) \<noteq> {}"
+    \<comment> \<open>Any two sets that intersect @{term \<open>I\<^sub>1\<union>I\<^sub>2\<close>} and that are quorums in the system projected on @{term \<open>I\<^sub>1\<union>I\<^sub>2\<close>} intersect in @{term \<open>I\<^sub>1\<union>I\<^sub>2\<close>}.\<close>
+proof -
+  text \<open>First we show that @{term Q\<^sub>1} and @{term Q\<^sub>2} are quorums in the projections on @{term I\<^sub>1} and @{term I\<^sub>2}.\<close>
+  have "i1.proj.quorum Q\<^sub>1" using \<open>proj.quorum Q\<^sub>1\<close> 
+    unfolding i1.proj.quorum_def proj.quorum_def project_def
+    by auto (metis Int_Un_distrib Int_iff Un_subset_iff) 
+  moreover have "i2.proj.quorum Q\<^sub>2" using \<open>proj.quorum Q\<^sub>2\<close> 
+    unfolding i2.proj.quorum_def proj.quorum_def project_def
+    by auto (metis Int_Un_distrib Int_iff Un_subset_iff) 
+  moreover have "i2.proj.quorum Q\<^sub>1" using \<open>proj.quorum Q\<^sub>1\<close>
+    unfolding proj.quorum_def i2.proj.quorum_def project_def
+    by auto (metis Int_Un_distrib Int_iff Un_subset_iff) 
+  moreover have "i1.proj.quorum Q\<^sub>2" using \<open>proj.quorum Q\<^sub>2\<close>
+    unfolding proj.quorum_def i1.proj.quorum_def project_def
+    by auto (metis Int_Un_distrib Int_iff Un_subset_iff) 
+  text \<open>Next we show that @{term Q\<^sub>1} and @{term Q\<^sub>2} intersect if they are quorums of, respectively, @{term I\<^sub>1} and @{term I\<^sub>2}. 
+This is the only interesting part of the proof.\<close> 
+  moreover have "Q\<^sub>1 \<inter> Q\<^sub>2 \<inter> (I\<^sub>1\<union>I\<^sub>2) \<noteq> {}" 
+    if "i1.proj.quorum Q\<^sub>1" and "i2.proj.quorum Q\<^sub>2" and "i2.proj.quorum Q\<^sub>1"
+      and "Q\<^sub>1 \<inter> I\<^sub>1 \<noteq> {}" and "Q\<^sub>2 \<inter> I\<^sub>2 \<noteq> {}"
+    for Q\<^sub>1 Q\<^sub>2
+  proof -
+    have "i1.proj.quorum I\<^sub>2" 
+    proof -
+      have "i1.orig.quorum I\<^sub>2" by (simp add: i2.q_avail)
+      thus ?thesis unfolding i1.orig.quorum_def i1.proj.quorum_def project_def
+        by auto (meson Int_commute Int_iff inf_le2 subset_trans)
+    qed
+    moreover note \<open>i1.proj.quorum Q\<^sub>1\<close>
+    ultimately have "Q\<^sub>1 \<inter> I\<^sub>2 \<noteq> {}" using i1.q_inter inter \<open>Q\<^sub>1 \<inter> I\<^sub>1 \<noteq> {}\<close> by blast
+
+    moreover note \<open>i2.proj.quorum Q\<^sub>2\<close>  
+    moreover note \<open>i2.proj.quorum Q\<^sub>1\<close>
+    ultimately have "Q\<^sub>1 \<inter> Q\<^sub>2 \<inter> I\<^sub>2 \<noteq> {}" using i2.q_inter \<open>Q\<^sub>2 \<inter> I\<^sub>2 \<noteq> {}\<close> by blast 
+    thus ?thesis by (simp add: inf_sup_distrib1)
+  qed
+  text \<open>Next  we show that @{term Q\<^sub>1} and @{term Q\<^sub>2} intersect if they are quorums of the same intact set. This is obvious.\<close>
+  moreover
+  have "Q\<^sub>1 \<inter> Q\<^sub>2 \<inter> (I\<^sub>1\<union>I\<^sub>2) \<noteq> {}" 
+    if "i1.proj.quorum Q\<^sub>1" and "i1.proj.quorum Q\<^sub>2" and "Q\<^sub>1 \<inter> I\<^sub>1 \<noteq> {}" and "Q\<^sub>2 \<inter> I\<^sub>1 \<noteq> {}"
+    for Q\<^sub>1 Q\<^sub>2
+    by (simp add: Int_Un_distrib i1.q_inter that)  
+  moreover
+  have "Q\<^sub>1 \<inter> Q\<^sub>2 \<inter> (I\<^sub>1\<union>I\<^sub>2) \<noteq> {}"
+    if "i2.proj.quorum Q\<^sub>1" and "i2.proj.quorum Q\<^sub>2" and "Q\<^sub>1 \<inter> I\<^sub>2 \<noteq> {}" and "Q\<^sub>2 \<inter> I\<^sub>2 \<noteq> {}"
+    for Q\<^sub>1 Q\<^sub>2
+    by (simp add: Int_Un_distrib i2.q_inter that)
+  text \<open>Finally we have covered all the cases and get the final result:\<close>
+  ultimately
+  show ?thesis
+    by (smt Int_Un_distrib Int_commute assms(3,4) sup_bot.right_neutral) 
 qed
 
 end
